messageInvariantPrototypes/paxos/centralized/system.dfy
@@ -1,0 +1,180 @@
+include "hosts.dfy"
+
+module System {
+  import opened UtilitiesLibrary
+  import opened Types
+  import LeaderHost
+  import AcceptorHost
+  import LearnerHost
+
+datatype Constants = Constants(
+  f: nat,
+  leaderConstants: seq<LeaderHost.Constants>,
+  acceptorConstants: seq<AcceptorHost.Constants>,
+  learnerConstants: seq<LearnerHost.Constants>
+)
+{
+  ghost predicate WF() {
+    && 0 < f
+    && UniqueIds()
+  }
+  
+  ghost predicate UniqueIds() {
+    && UniqueLeaderIds()
+    && UniqueAcceptorIds()
+    && UniqueLearnerIds()
+  }
+
+  ghost predicate ValidLeaderIdx(id: int) {
+    0 <= id < |leaderConstants|
+  }
+
+  ghost predicate ValidAcceptorIdx(id: int) {
+    0 <= id < |acceptorConstants|
+  }
+
+  ghost predicate ValidLearnerIdx(id: int) {
+    0 <= id < |learnerConstants|
+  }
+  
+  ghost predicate UniqueLeaderIds() {
+    forall i, j | ValidLeaderIdx(i) && ValidLeaderIdx(j) && leaderConstants[i].id == leaderConstants[j].id :: i == j
+  }
+
+  ghost predicate UniqueAcceptorIds() {
+    forall i, j | ValidAcceptorIdx(i) && ValidAcceptorIdx(j) && acceptorConstants[i].id == acceptorConstants[j].id :: i == j
+  }
+
+  ghost predicate UniqueLearnerIds() {
+    forall i, j | ValidLearnerIdx(i) && ValidLearnerIdx(j) && learnerConstants[i].id == learnerConstants[j].id :: i == j
+  }
+} // end datatype Constants
+
+datatype Variables = Variables(
+  leaders: seq<LeaderHost.Variables>,
+  acceptors: seq<AcceptorHost.Variables>,
+  learners: seq<LearnerHost.Variables>
+)
+{
+  ghost predicate WF(c: Constants) {
+    && c.WF()
+    && LeaderHost.GroupWF(c.leaderConstants, leaders, c.f)
+    && AcceptorHost.GroupWF(c.acceptorConstants, acceptors, c.f)
+    && LearnerHost.GroupWF(c.learnerConstants, learners, c.f)
+  }
+} // end datatype Variables
+
+
+//// System Transitions ////
+
+ghost predicate Init(c: Constants, v: Variables) {
+  && v.WF(c)
+  && LeaderHost.GroupInit(c.leaderConstants, v.leaders, c.f)
+  && AcceptorHost.GroupInit(c.acceptorConstants, v.acceptors, c.f)
+  && LearnerHost.GroupInit(c.learnerConstants, v.learners, c.f)
+}
+
+datatype Step = 
+  | P1aStep(leader: LeaderId, acceptor: AcceptorId)
+  | P1bStep(acceptor: AcceptorId, leader: LeaderId, balOpt:Option<LeaderId>, vbOptOpt:Option<Option<ValBal>>)
+  | P2aStep(leader: LeaderId, acceptor: AcceptorId, val: Value)
+  | P2bStep(acceptor: AcceptorId, learner: LearnerId, vbOpt: Option<ValBal>)
+  | StutterStep()
+
+ghost predicate NextP1aStep(c: Constants, v: Variables, v': Variables, ldr: LeaderId, acc: AcceptorId) 
+  requires v.WF(c) && v'.WF(c)
+{
+  var ldrLbl := LeaderHost.InternalLbl();
+  var accLbl := AcceptorHost.ReceivePrepareLbl(ldr);
+  && c.ValidLeaderIdx(ldr)
+  && c.ValidAcceptorIdx(acc)
+  && AcceptorHost.Next(c.acceptorConstants[acc], v.acceptors[acc], v'.acceptors[acc], accLbl)
+  && AcceptorsUnchangedExcept(c, v, v', acc)
+  && LeadersUnchanged(v, v')
+  && LearnersUnchanged(v, v')
+}
+
+ghost predicate NextP1bStep(c: Constants, v: Variables, v': Variables, 
+    ldr: LeaderId, acc: AcceptorId,
+    balOpt: Option<LeaderId>, vbOptOpt: Option<Option<ValBal>>) 
+  requires v.WF(c) && v'.WF(c)
+{
+  var accLbl := AcceptorHost.MaybePromiseLbl(balOpt, vbOptOpt);
+  && c.ValidLeaderIdx(ldr)
+  && c.ValidAcceptorIdx(acc)
+  && AcceptorHost.Next(c.acceptorConstants[acc], v.acceptors[acc], v'.acceptors[acc], accLbl)
+  && AcceptorsUnchangedExcept(c, v, v', acc)
+  && LearnersUnchanged(v, v')
+  && if balOpt.Some? then
+        && assert vbOptOpt.Some?;  // Tony: I am surprised Dafny sees this
+        && var ldrLbl := LeaderHost.ReceivePromiseLbl(acc, vbOptOpt.value);
+        && ldr == balOpt.value
+        && LeaderHost.Next(c.leaderConstants[ldr], v.leaders[ldr], v'.leaders[ldr], ldrLbl)
+        && LeadersUnchangedExcept(c, v, v', ldr)
+      else 
+        LeadersUnchanged(v, v')
+}
+
+
+
+
+
+ghost predicate NextStep(c: Constants, v: Variables, v': Variables, step: Step)
+  requires v.WF(c) && v'.WF(c)
+{
+  match step
+    case P1aStep(ldr, acc) => NextP1aStep(c, v, v', ldr, acc)
+    case P1bStep(acc, ldr, balOpt, vbOptOpt) => NextP1bStep(c, v, v', acc, ldr, balOpt, vbOptOpt)
+    case P2aStep(ldr, acc, val) => v' == v
+    case P2bStep(acc, lnr, vbOpt) => v' == v
+    case StutterStep => v' == v
+}
+
+ghost predicate Next(c: Constants, v: Variables, v': Variables)
+{
+  && v.WF(c)
+  && v'.WF(c)
+  && exists step :: NextStep(c, v, v', step)
+}
+
+
+//// Helper Functions ////
+
+ghost predicate LeadersUnchanged(v: Variables, v': Variables) {
+  v'.leaders == v.leaders
+}
+
+ghost predicate LeadersUnchangedExcept(c: Constants, v: Variables, v': Variables, ldr: LeaderId)
+  requires v.WF(c) && v'.WF(c)
+  requires c.ValidLeaderIdx(ldr)
+{
+  forall id:nat | c.ValidLeaderIdx(id) && id != ldr
+  :: v.leaders[id] == v'.leaders[id]
+}
+
+ghost predicate AcceptorsUnchanged(v: Variables, v': Variables) {
+  v'.acceptors == v.acceptors
+}
+
+ghost predicate AcceptorsUnchangedExcept(c: Constants, v: Variables, v': Variables, acc: AcceptorId)
+  requires v.WF(c) && v'.WF(c)
+  requires c.ValidAcceptorIdx(acc)
+{
+  forall id:nat | c.ValidAcceptorIdx(id) && id != acc
+  :: v.acceptors[id] == v'.acceptors[id]
+}
+
+ghost predicate LearnersUnchanged(v: Variables, v': Variables) {
+  v'.learners == v.learners
+}
+
+ghost predicate LearnersUnchangedExcept(c: Constants, v: Variables, v': Variables, lnr: LearnerId)
+  requires v.WF(c) && v'.WF(c)
+  requires c.ValidLearnerIdx(lnr)
+{
+  forall id:nat | c.ValidLearnerIdx(id) && id != lnr
+  :: v.learners[id] == v'.learners[id]
+}
+
+
+} // end module System
